src/trace/coqTerms.ml
@@ -161,6 +161,7 @@ let cUO_Zneg = gen_constant smt_modules "UO_Zneg"
 let cUO_Zopp = gen_constant smt_modules "UO_Zopp"
 let cUO_BVbitOf = gen_constant smt_modules "UO_BVbitOf"
 let cUO_BVnot = gen_constant smt_modules "UO_BVnot"
+let cUO_BVneg = gen_constant smt_modules "UO_BVneg"
 
 let cBO_Zplus = gen_constant smt_modules "BO_Zplus"
 let cBO_Zminus = gen_constant smt_modules "BO_Zminus"
@@ -216,7 +217,7 @@ let make_certif_ops modules args =
   gen_constant "LiaMicromega", gen_constant "LiaDiseq", gen_constant "SplArith", gen_constant "SplDistinctElim",
   gen_constant "BBVar", gen_constant "BBConst",
   gen_constant "BBOp", gen_constant "BBNot", gen_constant "BBEq",
-  gen_constant "BBAdd", gen_constant "BBMul",
+  gen_constant "BBNeg", gen_constant "BBAdd", gen_constant "BBMul",
   gen_constant "Hole")
   
 
