src/SMT_terms.v
@@ -587,7 +587,8 @@ Module Atom.
    | UO_Zneg
    | UO_Zopp
    | UO_BVbitOf (_: N) (_: nat)
-   | UO_BVnot (_: N).
+   | UO_BVnot (_: N)
+   | UO_BVneg (_: N).
 
   Inductive binop : Type :=
    | BO_Zplus
@@ -640,6 +641,7 @@ Module Atom.
    | UO_Zopp, UO_Zopp => true
    | UO_BVbitOf s1 n, UO_BVbitOf s2 m => Nat_eqb n m && N.eqb s1 s2
    | UO_BVnot s1, UO_BVnot s2 => N.eqb s1 s2
+   | UO_BVneg s1, UO_BVneg s2 => N.eqb s1 s2
    | _,_ => false
    end.
 
@@ -821,6 +823,7 @@ Qed.
         | UO_Zopp => (Typ.TZ, Typ.TZ)
         | UO_BVbitOf s _ => (Typ.TBV, Typ.Tbool)
         | UO_BVnot s => (Typ.TBV, Typ.TBV)
+        | UO_BVneg s => (Typ.TBV, Typ.TBV)
         end.
 
       Definition typ_bop o := 
@@ -959,6 +962,14 @@ Qed.
          (case (Typ.eqb (get_type h) (Typ.TBV))).
           left. exists Typ.Tbool. easy.
           right. intros. rewrite andb_false_r. easy.
+
+         (case (Typ.eqb (get_type h) Typ.TBV)).
+           left. exists Typ.TBV. easy.
+           right. intros. rewrite andb_false_r. easy.
+         
+         (case (Typ.eqb (get_type h) Typ.TBV)).
+           left. exists Typ.TBV. easy.
+           right. intros. rewrite andb_false_r. easy.
 
          (case (Typ.eqb (get_type h) Typ.TBV)).
            left. exists Typ.TBV. easy.
@@ -1114,6 +1125,7 @@ Qed.
         | UO_Zopp => apply_unop Typ.TZ Typ.TZ Zopp
         | UO_BVbitOf s n => apply_unop Typ.TBV Typ.Tbool (BITVECTOR_LIST_FIXED.bitOf n)
         | UO_BVnot s => apply_unop Typ.TBV Typ.TBV BITVECTOR_LIST_FIXED.bv_not
+        | UO_BVneg s => apply_unop Typ.TBV Typ.TBV BITVECTOR_LIST_FIXED.bv_neg
         end.
 
       Definition interp_bop o :=
@@ -1303,6 +1315,7 @@ Qed.
         exists (- y)%Z; auto.
         exists (BITVECTOR_LIST_FIXED.bitOf n0 y); auto.
         exists (BITVECTOR_LIST_FIXED.bv_not y); auto.
+        exists (BITVECTOR_LIST_FIXED.bv_neg y); auto.
 
   (* Binary operators *)
         destruct op as [ | | | | | | | A |s1|s2| s3 | s4 | s5 | s6 ]; intros [i | | | |s]; 
@@ -1540,6 +1553,7 @@ Qed.
             try (pose (H2 := H Typ.Tpositive); simpl in H2; rewrite H2; auto);
             try (pose (H2 := H Typ.TZ); simpl in H2; rewrite H2; auto);
             try (pose (H2 := H Typ.Tbool); simpl in H2; rewrite H2; auto);
+            try (pose (H2 := H Typ.TBV); simpl in H2; rewrite H2; auto);
             pose (H2 := H Typ.TBV); simpl in H2; rewrite H2; auto.
         (* Binary operators *)
         destruct op; simpl; intro H; destruct (check_aux_interp_hatom h1) as [v1 Hv1]; 
@@ -1771,7 +1785,7 @@ Qed.
         exists 0%Z; auto.
         exists (BITVECTOR_LIST_FIXED.of_bits l); auto.
         (* Unary operators *)
-        intros [ | | | | | | ] i H; simpl; destruct (IH i H) as [x Hx]; rewrite Hx; simpl.
+        intros [ | | | | | | | ] i H; simpl; destruct (IH i H) as [x Hx]; rewrite Hx; simpl.
         case (Typ.cast (v_type Typ.type interp_t (a .[ i])) Typ.Tpositive); simpl; try (exists true; auto); intro k; exists ((k interp_t x)~0)%positive; auto.
         case (Typ.cast (v_type Typ.type interp_t (a .[ i])) Typ.Tpositive); simpl; try (exists true; auto); intro k; exists ((k interp_t x)~1)%positive; auto.
         case (Typ.cast (v_type Typ.type interp_t (a .[ i])) Typ.Tpositive); simpl; try (exists true; auto); intro k; exists (Zpos (k interp_t x)); auto.
@@ -1779,6 +1793,7 @@ Qed.
         case (Typ.cast (v_type Typ.type interp_t (a .[ i])) Typ.TZ); simpl; try (exists true; auto); intro k; exists (- k interp_t x)%Z; auto.
         case (Typ.cast (v_type Typ.type interp_t (a .[ i])) Typ.TBV); simpl; [ | exists true; auto]. intro k; exists (BITVECTOR_LIST_FIXED.bitOf n0 (k interp_t x)) ; auto.
         case (Typ.cast (v_type Typ.type interp_t (a .[ i])) Typ.TBV); simpl; [ | exists true; auto]. intro k; exists (BITVECTOR_LIST_FIXED.bv_not (k interp_t x)) ; auto.
+        case (Typ.cast (v_type Typ.type interp_t (a .[ i])) Typ.TBV); simpl; [ | exists true; auto]. intro k; exists (BITVECTOR_LIST_FIXED.bv_neg (k interp_t x)) ; auto.
 
    (* Binary operators *)
         intros [ | | | | | | |A | | | | | | ] h1 h2; simpl; rewrite andb_true_iff; intros [H1 H2]; destruct (IH h1 H1) as [x Hx]; destruct (IH h2 H2) as [y Hy]; rewrite Hx, Hy; simpl.
