src/spl/Syntactic.v
@@ -123,19 +123,20 @@ Section CheckAtom.
       intros [op2|op2 i2|op2 i2 j2|op2 li2|f2 args2]; simpl; try discriminate; try (case op1; discriminate).
       case op1; case op2; try discriminate; try (unfold is_true; rewrite andb_true_iff; intros [_ H]; rewrite (check_hatom_correct _ _ H); auto).
 
-      case_eq (get_atom i2); try discriminate; intros [ | | | | | | ] i Heq H; try discriminate; simpl;
+      case_eq (get_atom i2); try discriminate; intros [ | | | | | | | ] i Heq H; try discriminate; simpl;
       unfold apply_unop; rewrite (check_hatom_correct _ _ H); 
       unfold interp_hatom; rewrite (t_interp_wf _ _ _ Hwf Hd i2), Heq; simpl; 
       unfold apply_unop; destruct (t_interp t_i t_func t_atom .[ i]) as [A v]; 
       destruct (Typ.cast A Typ.Tpositive) as [k| ]; auto.
 
-      case_eq (get_atom i1); try discriminate; intros [ | | | | | | ] i Heq H; try discriminate; simpl; 
+      case_eq (get_atom i1); try discriminate; intros [ | | | | | | | ] i Heq H; try discriminate; simpl; 
       unfold apply_unop. rewrite <- (check_hatom_correct _ _ H); 
       unfold interp_hatom; rewrite (t_interp_wf _ _ _ Hwf Hd i1), Heq; simpl; 
       unfold apply_unop; destruct (t_interp t_i t_func t_atom .[ i]) as [A v]; 
       destruct (Typ.cast A Typ.Tpositive) as [k| ]; auto.
 
       intros n m n1 m2. simpl. unfold is_true. rewrite !andb_true_iff, beq_nat_true_iff, N.eqb_eq. intros [[-> ->] H]. rewrite (check_hatom_correct _ _ H); auto.
+      intros n m. simpl. unfold is_true. rewrite andb_true_iff, N.eqb_eq. intros [-> H]. rewrite (check_hatom_correct _ _ H); auto.
       intros n m. simpl. unfold is_true. rewrite andb_true_iff, N.eqb_eq. intros [-> H]. rewrite (check_hatom_correct _ _ H); auto.
             (* Binary operators *)
       - intros [op2|op2 i2|op2 i2 j2|op2 li2|f2 args2]; simpl; try discriminate; case op1; case op2; try discriminate; try (unfold is_true; rewrite andb_true_iff; intros [H1 H2]; rewrite (check_hatom_correct _ _ H1), (check_hatom_correct _ _ H2); auto).
